\documentclass[12pt]{article}
\usepackage[utf8x]{inputenc}
\usepackage[english]{babel}
\usepackage[T1]{fontenc}
\usepackage{color}
\usepackage{wrapfig}
\usepackage{amsmath}
\usepackage{amssymb}
\usepackage{textcomp}
\usepackage{array}
\usepackage{booktabs}
\usepackage{subfigure}
\usepackage[font=small,format=plain,labelfont=bf,up,textfont=it,up]{caption}
\usepackage{longtable}
\usepackage{calc}
\usepackage{setspace}
\usepackage{multirow}
\usepackage{hhline}
\usepackage{ifthen}
\usepackage{lscape}
\usepackage{relsize}
\usepackage{bbold}
\usepackage{mathtext}
\usepackage{pdfpages}
\usepackage{geometry}
 \geometry{
 a4paper,
 total={170mm,257mm},
 left=35mm,
 top=25mm,
 bottom=25mm,
 right=20mm,
 }
\usepackage{cite}
\linespread{1.3}

\begin{document}
\begin{equation}
i\partial \psi_{i} = [ F_{\psi_i}+V(t)]
\text{\ \ \ \ \ \ }
\psi_{i}(t) = d^{i}_{mn}(t) e^{{i\epsilon_{m}t}}\overline{\psi}_{m}
\text{\ \ \ \ \ \ }
F_{0} \psi_{p} = \epsilon_{p}\overline{\psi}_{p}
\end{equation}
\begin{equation}
i\dot{d}^{i}_{m} = ( F_{nm} - \delta_{nm}\epsilon +V_{mn})d_{m}^{i}e^{i(\epsilon_{n}-\epsilon_{m}})t  
\end{equation}

\begin{equation}
X_{nm} = \langle \psi_{n} | \hat{X} | \psi_{m} \rangle 
\end{equation}
\begin{equation}
\langle \overline{\psi}_{p} | \overline{\psi}_{q} \rangle = \delta_{pq}
\end{equation}
\begin{equation}
i\dot{d}_{m}^{0i} = 0 
\text{\ \ \ \ \ \ }
\psi_{i}(t_{0}) = d^{0i}_{m}\overline{\psi}_{m}
\text{\ \ \ \ \ \ }
\psi_{i}(t_{0}) = d^{0i}_{m} \neq \delta_{mi}
\end{equation}
\begin{equation}
i\dot{d}_{m}^{1i} = ( F_{nm}^{1} + V_{nm}^{1}) d_{m}^{0i} e^{i(\epsilon_{n}-\epsilon_{m})}t
\end{equation}
\begin{equation}
\rho_{k} = \psi^{\dagger}_{i}\Sigma_{k}\psi_{i} = 
d^{i*}_{l}d_{s}^{i}e^{i(\epsilon_{l}-\epsilon_{s})}t \overline{\Psi}_{l}^{\dagger}\Sigma_{k}\overline{psi}_{s}
\end{equation}
\begin{equation}
\rho_{k} = D_{sl}e^{i(\epsilon_{l}-\epsilon_{s})t}\Omega^{k}_{ls} 
\end{equation}
\begin{equation}
\nabla \rho_{k} = D_{sk} e^{i(\epsilon_{l}-\epsilon_{s})t} \nabla \Omega_{ls}^{k}
\end{equation}
\begin{equation}
F_{nm}^{1} = \frac{d F_{nm}}{d D_{sl} } D^{1}_{sl}
= \frac{d \tilde{F}_{nm}}{d D_{sl} } e^{i(\epsilon_{j}-\epsilon_{s})t}((d_{l}^{0j})^{*} d_{s}^{1j} + (d_{l}^{1j})^{*} d_{s}^{0j} ) 
\end{equation}
\begin{equation}
F_{nm}^{1} d_{m}^{0i} = F_{mi}^{1} =
 K_{mi,sj} e^{i(\epsilon_{j}-\epsilon_{s})t}d_{s}^{1j} +
 K_{mi,jl} e^{i(\epsilon_{l}-\epsilon_{j})t}(d_{s}^{1j})^{*}
\end{equation}
\begin{equation} 
K_{mm, ls} = \frac{d \tilde{F}_{nm}}{d D_{sl}}
\end{equation}
\begin{equation}
i\dot{d}^{1i}_{m} = 
( K_{mi,lj} e^{i(\epsilon_{j} -\epsilon_{l})t}) +
( K_{mi,jl} e^{i(\epsilon_{l} -\epsilon_{j})t})(d_{l}^{1j})^{*}
\end{equation}
\begin{equation}
i\dot{d}^{1i}_{m} = \tilde{d}^{1i}_{m}e^{-i(\epsilon_{i}-\epsilon_{m})t}
( K_{mi,lj} e^{i(\epsilon_{j} -\epsilon_{l})t}) +
( K_{mi,jl} e^{i(\epsilon_{l} -\epsilon_{j})t})(d_{l}^{1j})^{*}
\end{equation}

\end{document}
